CacheLocal.v
@@ -1,0 +1,22 @@
+Require Import DataTypes Coherence Tree.
+
+Module mkCacheLocal (coh: Coherence).
+  Record CacheState :=
+    {
+      state: Tree -> Addr -> coh.t;
+      dir: Tree -> Tree -> Addr -> coh.t;
+      data: Tree -> Addr -> Data;
+      wait: Tree -> Addr -> bool;
+      waitS: Tree -> Addr -> coh.t;
+      dwait: Tree -> Tree -> Addr -> bool;
+      dwaitS: Tree -> Tree -> Addr -> coh.t;
+      next: Tree -> nat
+    }.
+
+  Record CacheLocal :=
+    {
+      getCacheState: Time -> CacheState;
+      deqR: Proc -> Time -> Prop
+    }.
+
+End mkCacheLocal.
