Coherence.v
@@ -1,0 +1,191 @@
+Require Import Coq.Structures.Orders Coq.Structures.OrdersTac.
+
+Module Type Coherence.
+  Parameter t: Set.
+  Parameter Mo Sh In: t.
+
+  Definition eq (x y: t) := x = y.
+  Parameter lt: t -> t -> Prop.
+  Definition le (x y: t) := lt x y \/ x = y.
+
+  Axiom eq_equiv: Equivalence eq.
+  Axiom lt_strorder: StrictOrder lt.
+  Axiom lt_compat: Proper (eq ==> eq ==> iff) lt.
+  Axiom le_lteq: forall x y, le x y <-> lt x y \/ eq x y.
+  Axiom lt_total: forall x y, lt x y \/ eq x y \/ lt y x.
+  Axiom maxMo: forall x, le x Mo.
+  Axiom maxMo': forall x, lt Mo x -> False.
+  Axiom minIn: forall x, le In x.
+  Axiom minIn': forall x, lt x In -> False.
+
+  Parameter compatible: t -> t -> Prop.
+End Coherence.
+
+Ltac coherence := repeat match goal with
+                           | [|- context [?fn]] => unfold fn
+                           | [H: context [?fn] |- _] => unfold fn in H
+                           | [|- forall x, _] => intro
+                           | [H: ?x = ?y |- _] => rewrite H in *
+                           | [x: ?P |- _] => destruct x
+                         end; auto; try discriminate.
+
+
+Module Msi <: Coherence.
+  Inductive State := Mod | Sha | Inv.
+
+  Definition t := State.
+
+  Definition Mo := Mod.
+  Definition Sh := Sha.
+  Definition In := Inv.
+
+  Definition eq (x y : t) := x = y.
+  Definition lt (x y : t) := match x, y with
+                               | In, In => False
+                               | In, _ => True
+                               | Sh, Mo => True
+                               | Sh, _ => False
+                               | Mo, _ => False
+                             end.
+  Definition le (x y : t) := lt x y \/ x = y.
+
+  Theorem eq_equiv: Equivalence eq.
+  Proof.
+    constructor; coherence.
+  Qed.
+
+  Theorem lt_strorder: StrictOrder lt.
+  Proof.
+    constructor; coherence.
+  Qed.
+
+  Theorem lt_compat: Proper (eq ==> eq ==> iff) lt.
+  Proof.
+    constructor; coherence.
+  Qed.
+
+  Theorem le_lteq: forall x y, le x y <-> lt x y \/ eq x y.
+  Proof.
+    constructor; coherence.
+  Qed.
+
+  Theorem lt_total: forall x y, lt x y \/ eq x y \/ lt y x.
+  Proof.
+    coherence.
+  Qed.
+
+  Theorem maxMo: forall x, le x Mo.
+  Proof.
+    coherence.
+  Qed.
+
+  Theorem maxMo': forall x, lt Mo x -> False.
+  Proof.
+    coherence.
+  Qed.
+
+  Theorem minIn: forall x, le In x.
+  Proof.
+    coherence.
+  Qed.
+
+  Theorem minIn': forall x, lt x In -> False.
+  Proof.
+    coherence.
+  Qed.
+
+  Definition compatible x y :=
+    match x, y with
+      | In, _ => True
+      | Sh, Mo => False
+      | Sh, _ => True
+      | Mo, In => True
+      | Mo, _ => False
+    end.
+
+  Hint Resolve maxMo maxMo' minIn minIn'.
+  Hint Unfold compatible.
+End Msi.
+
+Module Mosi <: Coherence.
+  Inductive State := Mod | Ow | Sha | Inv.
+
+  Definition t := State.
+
+  Definition Mo := Mod.
+  Definition Sh := Sha.
+  Definition In := Inv.
+
+  Definition eq (x y : t) := x = y.
+  Definition lt (x y : t) := match x, y with
+                               | In, In => False
+                               | In, _ => True
+                               | Sh, Mo => True
+                               | Sh, Ow => True
+                               | Sh, _ => False
+                               | Ow, Mo => True
+                               | Ow, _ => False
+                               | Mo, _ => False
+                             end.
+  Definition le (x y : t) := lt x y \/ x = y.
+
+  Theorem eq_equiv: Equivalence eq.
+  Proof.
+    constructor; coherence.
+  Qed.
+
+  Theorem lt_strorder: StrictOrder lt.
+  Proof.
+    constructor; coherence.
+  Qed.
+
+  Theorem lt_compat: Proper (eq ==> eq ==> iff) lt.
+  Proof.
+    constructor; coherence.
+  Qed.
+
+  Theorem le_lteq: forall x y, le x y <-> lt x y \/ eq x y.
+  Proof.
+    constructor; coherence.
+  Qed.
+
+  Theorem lt_total: forall x y, lt x y \/ eq x y \/ lt y x.
+  Proof.
+    coherence.
+  Qed.
+
+  Theorem maxMo: forall x, le x Mo.
+  Proof.
+    coherence.
+  Qed.
+
+  Theorem maxMo': forall x, lt Mo x -> False.
+  Proof.
+    coherence.
+  Qed.
+
+  Theorem minIn: forall x, le In x.
+  Proof.
+    coherence.
+  Qed.
+
+  Theorem minIn': forall x, lt x In -> False.
+  Proof.
+    coherence.
+  Qed.
+
+  Definition compatible x y :=
+    match x, y with
+      | In, _ => True
+      | Sh, Mo => False
+      | Sh, _ => True
+      | Ow, Mo => False
+      | Ow, Ow => False
+      | Ow, _ => True
+      | Mo, In => True
+      | Mo, _ => False
+    end.
+
+  Hint Resolve maxMo maxMo' minIn minIn'.
+  Hint Unfold compatible.
+End Mosi.
