FirstLevel.v
@@ -1,0 +1,71 @@
+Require Import StoreAtomicity Coherence CacheLocal Tree DataTypes.
+
+Set Implicit Arguments.
+
+Module FirstLevel (coh: Coherence).
+  Module mkCl := mkCacheLocal coh.
+  Import coh mkCl.
+  Section GivenState.
+    Variable t: Time.
+    Variable a: Addr.
+    Variable respFn: nat -> option Resp.
+
+    Variable cl: CacheLocal.
+
+    Definition s := getCacheState cl t.
+    Definition nextS := getCacheState cl (S t).
+
+    Definition clean p :=
+      le Sh (state s p a) /\ forall c, parent c p -> le (dir s p c a) Sh.
+
+    Record FirstLevel :=
+      {
+        latestValue:
+          forall pCache,
+            let p := node pCache in
+            clean p ->
+            (data s p a = initData a /\
+             forall t', t' < t -> noStore respFn t' a ) \/
+            (exists tm,
+               tm < t /\
+               match respFn tm with
+                 | Some (Build_Resp cm im dm) =>
+                   let (am, descQm, dtQm) := reqFn cm im in
+                   data s p a = dtQm /\ am = a /\ descQm = St /\
+                   forall t', tm < t' < t -> noStore respFn t' a
+                 | None => False
+               end);
+
+        nonAncestorCompatible:
+          forall cCache1 cCache2: Cache,
+            let c1 := node cCache1 in
+            let c2 := node cCache2 in
+            ~ descendent c1 c2 ->
+            ~ descendent c2 c1 ->
+            compatible (state s c1 a) (state s c2 a);
+
+        processReq:
+          forall cProc,
+            deqR cl cProc t ->
+            let c := p_node cProc in
+            let (a, op, d) := reqFn cProc (next s c) in
+            match op with
+              | Ld => le Sh (state s c a)
+              | St => state s c a = Mo
+            end;
+
+        nextChange:
+          forall cProc,
+            let c := p_node cProc in
+            next nextS c <> next s c ->
+            deqR cl cProc t;
+
+        noReqAgain:
+          forall cProc,
+            let c := p_node cProc in
+            deqR cl cProc t ->
+            next nextS c = S (next s c)
+            
+      }.
+  End GivenState.
+End FirstLevel.
