StoreAtomicity.v
@@ -2,66 +2,64 @@ Require Import DataTypes.
 
 Set Implicit Arguments.
 
-Record StoreAtomic (respFn: nat -> option Resp) :=
-  {
-    uniqRespLabels:
-      forall t1 t2, match respFn t1, respFn t2 with
-                      | Some (Build_Resp c1 i1 _), Some (Build_Resp c2 i2 _) =>
-                        p_node c1 = p_node c2 -> i1 = i2 -> t1 = t2
-                      | _, _ => True
-                    end;
+Section StoreAtomicity.
+  Variable respFn: Time -> option Resp.
+  Definition noStore t a :=
+    match respFn t with
+      | Some (Build_Resp c' i' d') =>
+        let (a', descQ', dtQ') := reqFn c' i' in
+        a' = a -> descQ' = St -> False
+      | _ => True
+    end.
 
-    localOrdering:
-      forall t1 t2, match respFn t1, respFn t2 with
-                      | Some (Build_Resp c1 i1 _), Some (Build_Resp c2 i2 _) =>
-                        p_node c1 = p_node c2 -> i1 > i2 -> t1 > t2
-                      | _, _ => True
-                    end;
+  Record StoreAtomicity :=
+    {
+      uniqRespLabels:
+        forall t1 t2, match respFn t1, respFn t2 with
+                        | Some (Build_Resp c1 i1 _), Some (Build_Resp c2 i2 _) =>
+                          p_node c1 = p_node c2 -> i1 = i2 -> t1 = t2
+                        | _, _ => True
+                      end;
 
-    allPrevious:
-      forall t2, match respFn t2 with
-                   | Some (Build_Resp c2 i2 _) =>
-                     forall i1, i1 < i2 -> exists t1, t1 < t2 /\
-                                                      match respFn t1 with
-                                                        | Some (Build_Resp c1 i _) =>
-                                                          p_node c1 = p_node c2 /\ i = i1
-                                                        | None => False
-                                                      end
-                   | _ => True
-                 end;
+      localOrdering:
+        forall t1 t2, match respFn t1, respFn t2 with
+                        | Some (Build_Resp c1 i1 _), Some (Build_Resp c2 i2 _) =>
+                          p_node c1 = p_node c2 -> i1 > i2 -> t1 > t2
+                        | _, _ => True
+                      end;
 
-    storeAtomicity:
-      forall t,
-        match respFn t with
-          | Some (Build_Resp c i d) =>
-            let (a, descQ, dtQ) := reqFn c i in
-            match descQ with
-              | Ld =>
-                (d = initData a /\
-                 forall t', t' < t ->
-                            match respFn t' with
-                              | Some (Build_Resp c' i' d') =>
-                                let (a', descQ', dtQ') := reqFn c' i' in
-                                a' = a -> descQ' = St -> False
-                              | _ => True
-                            end) \/
-                (exists tm,
-                   tm < t /\
-                   match respFn tm with
-                     | Some (Build_Resp cm im dm) =>
-                       let (am, descQm, dtQm) := reqFn cm im in
-                       d = dtQm /\ am = a /\ descQm = St /\
-                       forall t', tm < t' < t ->
-                                match respFn t' with
-                                  | Some (Build_Resp c' i' d') =>
-                                    let (a', descQ', dtQ') := reqFn c' i' in
-                                    a' = a -> descQ' = St -> False
-                                  | _ => True
-                                end
-                   | _ => False
-                   end)
-              | St => d = initData zero 
-            end
-          | _ => True
-        end
+      allPrevious:
+        forall t2, match respFn t2 with
+                     | Some (Build_Resp c2 i2 _) =>
+                       forall i1, i1 < i2 -> exists t1, t1 < t2 /\
+                                                        match respFn t1 with
+                                                          | Some (Build_Resp c1 i _) =>
+                                                            p_node c1 = p_node c2 /\ i = i1
+                                                          | None => False
+                                                        end
+                     | _ => True
+                   end;
+
+      storeAtomicity:
+        forall t,
+          match respFn t with
+            | Some (Build_Resp c i d) =>
+              let (a, descQ, dtQ) := reqFn c i in
+              match descQ with
+                | Ld =>
+                  (d = initData a /\ forall t', t' < t -> noStore t' a) \/
+                  (exists tm,
+                     tm < t /\
+                     match respFn tm with
+                       | Some (Build_Resp cm im dm) =>
+                         let (am, descQm, dtQm) := reqFn cm im in
+                         d = dtQm /\ am = a /\ descQm = St /\
+                         forall t', tm < t' < t -> noStore t' a
+                       | _ => False
+                     end)
+                | St => d = initData zero 
+              end
+            | _ => True
+          end
   }.
+End StoreAtomicity.
